Split tutorial files

tutorial/ex03-enums.lean
@@ -1,54 +1,6 @@
 /-
-Code from video https://youtu.be/S-aGjgIDQZY
+Similar to https://softwarefoundations.cis.upenn.edu/lf-current/Basics.html
 -/
-
-#eval "hello" ++ " " ++ "world"
-
-#eval (String.append "hello" " ").append "world"
-#eval ("hello".append " ").append "world"
-
-#check true
-
-def x := 10 -- x : Nat
-
-#check x + 2
-#eval x + 2
-
-def double (x : Int) := 2*x
-
-#check double
-#check (double)
-#eval double 3
-example : double 4 = 8 := rfl
-
----
-
-def twice (f : Nat → Nat) (a : Nat) := f (f a)
-
-#check twice
-#check (twice)
-
-#check (String.append)
-
---example: typeOf (String.append) = (String → String → String) := rfl
-example: (String -> String -> String) = (String → String → String) := rfl
-
-example: Nat = Nat := rfl
-
-example: ((Nat → Nat) → Nat → Nat) = ((Nat → Nat) -> (Nat → Nat)) := rfl
-
-#eval twice (fun x => x + 2) 10
-#eval twice (· + 2) 10
-
-def twicePlus2a := twice (fun x => x + 2)
-def twicePlus2b := twice (. + 2)
-#eval twicePlus2a 10
-#eval twicePlus2b 10
-
-theorem twice_add_2 (a : Nat) : twice (fun x => x + 2) a = a + 4 := rfl
-theorem twice_1 : twicePlus2a = twicePlus2b := rfl
-
----
 
 inductive Weekday where
   | sunday
