tutorial/ex01-hello.lean
@@ -1,0 +1,18 @@
+#eval "hello" ++ " " ++ "world"
+
+#eval (String.append "hello" " ").append "world"
+#eval ("hello".append " ").append "world"
+
+#check true
+
+def x := 10 -- x : Nat
+
+#check x + 2
+#eval x + 2
+
+def double (x : Int) := 2*x
+
+#check double
+#check (double)
+#eval double 3
+example : double 4 = 8 := rfl
