tutorial/ex02-functions.lean
@@ -1,0 +1,24 @@
+def twice (f : Nat → Nat) (a : Nat) := f (f a)
+
+#check twice
+#check (twice)
+
+#check (String.append)
+
+--example: typeOf (String.append) = (String → String → String) := rfl
+example: (String -> String -> String) = (String → String → String) := rfl
+
+example: Nat = Nat := rfl
+
+example: ((Nat → Nat) → Nat → Nat) = ((Nat → Nat) -> (Nat → Nat)) := rfl
+
+#eval twice (fun x => x + 2) 10
+#eval twice (· + 2) 10
+
+def twicePlus2a := twice (fun x => x + 2)
+def twicePlus2b := twice (. + 2)
+#eval twicePlus2a 10
+#eval twicePlus2b 10
+
+theorem twice_add_2 (a : Nat) : twice (fun x => x + 2) a = a + 4 := rfl
+theorem twice_1 : twicePlus2a = twicePlus2b := rfl
