tutorial/index.lean
@@ -1,0 +1,4 @@
+/-
+Tutorial video: https://youtu.be/S-aGjgIDQZY
+Code from https://github.com/leanprover/lean4/tree/master/doc/examples/Certora2022
+-/
